Get rid of traces

theories/stablesort.v
@@ -12,112 +12,48 @@ Unset Printing Implicit Defensive.
 
 Module StableSort.
 
-Section Traces.
+(* the type of polymorphic sort functions                                     *)
+Definition sort_ty :=
+  forall T : Type,                      (* the type of elements               *)
+    rel T ->                            (* the comparison function [leT]      *)
+    seq T ->                            (* input                              *)
+    seq T.                              (* output                             *)
 
-Variables (T : Type) (P : {pred T}) (leT : rel T).
+(* the type of sort functions abstracted over the type of sorted lists and    *)
+(* some operations on them, e.g., merge                                       *)
+Definition asort_ty :=
+  forall T : Type,                      (* the type of elements               *)
+  forall R : Type,                      (* the type of sorted lists           *)
+    rel T ->                            (* the comparison function [leT]      *)
+    (R -> R -> R) ->                    (* merge by [leT]                     *)
+    (R -> R -> R) ->                    (* merge by the converse of [leT]     *)
+    (T -> R) ->                         (* singleton sorted list              *)
+    R ->                                (* empty sorted list                  *)
+    seq T ->                            (* input                              *)
+    R.                                  (* output                             *)
 
-(* One easy way to prove the correctness of highly optimized stable sort      *)
-(* algorithms is to prove the equivalence between it and a simpler (but       *)
-(* unoptimized) algorithm, e.g., insertion sort. However, such equivalence    *)
-(* proof requires the comparison function [leT : rel T] to be total and       *)
-(* transitive so that [merge] is associative. These requirements are          *)
-(* undesirable since some correctness properties hold without them.           *)
-(* Therefore, we present a type of binary trees [trace] representing the      *)
-(* divide-and-conquer structure of sort. These trees can also be seen as      *)
-(* "traces" of sorting algorithms, and have to be balanced in the case of     *)
-(* O(n log n) mergesort. Nevertheless, these trees can also represent rather  *)
-(* naive algorithms such as insertion sort, since there is no such formal     *)
-(* "balanced" restriction.                                                    *)
-Inductive trace :=
-  | branch_trace   : bool -> trace -> trace -> trace
-  | leaf_trace b s : sorted (fun x y => leT x y == b) s -> trace.
-
-Definition empty_trace := @leaf_trace false [::] erefl.
-
-(* By flattening a trace, the input list can be obtained.                     *)
-Fixpoint flatten_trace (t : trace) : seq T :=
-  match t with
-    | branch_trace _ l r => flatten_trace l ++ flatten_trace r
-    | leaf_trace _ s _ => s
-  end.
-
-(* By sorting a trace, the output list can be obtained.                       *)
-Fixpoint sort_trace (t : trace) : seq T :=
-  match t with
-    | branch_trace true  l r => merge leT (sort_trace l) (sort_trace r)
-    | branch_trace false l r =>
-      rev (merge (fun x y => leT y x) (rev (sort_trace r)) (rev (sort_trace l)))
-    | leaf_trace true  s _ => s
-    | leaf_trace false s _ => rev s
-  end.
-
-Lemma all_trace (t : trace) : all P (sort_trace t) = all P (flatten_trace t).
-Proof.
-elim: t => [b l IHl r IHr|[] s] /=; rewrite ?all_rev //.
-by case: b; rewrite ?(all_rev, all_merge) all_cat IHl IHr // andbC.
-Qed.
-
-Lemma size_trace (t : trace) : size (sort_trace t) = size (flatten_trace t).
-Proof.
-elim: t => [b l IHl r IHr|[] s] /=; rewrite ?size_rev //.
-by case: b; rewrite ?(size_rev, size_merge, size_cat) IHl IHr // addnC.
-Qed.
-
-Lemma trace_nilp (t : trace) : nilp (sort_trace t) = nilp (flatten_trace t).
-Proof.
-by move: (sort_trace t) (flatten_trace t) (size_trace t) => [|? ?] [].
-Qed.
-
-Variant trace_nil_spec (t : trace) : seq T -> seq T -> bool -> bool -> Type :=
-  | TraceNil    : flatten_trace t = [::] -> sort_trace t = [::] ->
-                  trace_nil_spec t [::] [::] true true
-  | TraceNotNil : flatten_trace t <> [::] -> sort_trace t <> [::] ->
-                  trace_nil_spec t (flatten_trace t) (sort_trace t) false false.
-
-Lemma trace_nilP (t : trace) :
-  trace_nil_spec t (flatten_trace t) (sort_trace t)
-                 (nilp (flatten_trace t)) (nilp (sort_trace t)).
-Proof.
-case: nilP (trace_nilp t); case: nilP => //; last by constructor.
-by move=> /[dup] ? -> /[dup] ? ->; constructor.
-Qed.
-
-Definition trace_sort sort := forall s,
-   {t : trace | s = flatten_trace t & sort s = sort_trace t}.
-
-End Traces.
-
-Lemma perm_trace (T : eqType) (leT : rel T) (t : trace leT) :
-  perm_eql (sort_trace t) (flatten_trace t).
-Proof.
-apply/permPl; elim: t => [b l IHl r IHr|[] s _] //=; rewrite ?perm_rev //.
-by case: b; rewrite /= ?perm_rev perm_merge -?rev_cat ?perm_rev perm_cat.
-Qed.
-
-Parametricity Translation
-  (forall T : Type, rel T -> seq T -> seq T) as sort_ty_R.
+Parametricity sort_ty.
+Parametricity asort_ty.
 
 Structure function := Pack {
+  (* the sort function                                                        *)
   apply : forall T : Type, rel T -> seq T -> seq T;
-  (* Binary parametricity                                                     *)
-  (* _ : forall T1 T2 (T_R : T1 -> T2 -> Type)                                *)
-  (*            (leT1 : rel T1) (leT2 : rel T2),                              *)
-  (*     (forall (x1 : T1) (y1 : T2), T_R x1 y1 ->                            *)
-  (*      forall (x2 : T1) (y2 : T2), T_R x2 y2 ->                            *)
-  (*        bool_R (leT1 x1 x2) (leT2 y1 y2)) ->                              *)
-  (*     forall (xs : seq T1) (ys : seq T2),                                  *)
-  (*       list_R T_R xs ys -> list_R T_R (apply leT1 xs) (apply leT2 ys);    *)
-  _ : sort_ty_R apply apply;
-  (* Characterization by traces *)
-  _ : forall (T : Type) (leT : rel T), trace_sort leT (apply leT);
+  (* the *abstract* sort function                                             *)
+  asort : asort_ty;
+  (* the binary parametricity of [asort]                                      *)
+  _ : asort_ty_R asort asort;
+  (* [asort] instantiated with merge is extensionally equal to [apply]        *)
+  _ : forall T (leT : rel T),
+    let geT x y := leT y x in
+    asort leT (merge leT) (fun xs ys => rev (merge geT (rev ys) (rev xs)))
+      (fun x => [:: x]) [::]
+    =1 apply leT;
+  (* [asort] instantiated with concatenation is the identity function         *)
+  _ : forall T (leT : rel T), asort leT cat cat (fun x => [:: x]) [::] =1 id;
 }.
 
 Module Exports.
-Arguments leaf_trace {T leT} b s _.
-Arguments empty_trace {T leT}.
-Arguments flatten_trace {T leT} t.
-Arguments sort_trace {T leT} t.
-Arguments Pack apply _ _ : clear implicits.
+Arguments Pack apply asort _ _ _ : clear implicits.
 Notation stableSort := function.
 Notation StableSort := Pack.
 Coercion apply : function >-> Funclass.
@@ -126,44 +62,21 @@ End Exports.
 End StableSort.
 Export StableSort.Exports.
 
-Notation "[ tr]" := StableSort.empty_trace.
-Notation "[ 'tr<=' ]" := (StableSort.leaf_trace true [::] erefl)
-  (format "[ 'tr<=' ]").
-Notation "[ 'tr<=' x ]" := (StableSort.leaf_trace true [:: x] erefl)
-  (format "[ 'tr<='  x ]").
-
-Lemma trace2_subproof T (leT : rel T) (x y : T) :
-   sorted (fun x' y' => leT x' y' == leT x y) [:: x; y].
-Proof. by rewrite /= eqxx. Qed.
-
-Notation "[ 'tr' x1 ; x2 ]" :=
-  (StableSort.leaf_trace _ [:: x1; x2] (trace2_subproof _ x1 x2))
-  (format "[ 'tr'  x1 ;  x2 ]").
-
 (******************************************************************************)
 (* Merge functions                                                            *)
 (******************************************************************************)
 
-Module MergeR.
-Definition merge_ty := forall (T : Type) (leT : rel T), seq T -> seq T -> seq T.
-Parametricity merge_ty.
-End MergeR.
-
 (* The [MergeSig] and [RevmergeSig] module types are interfaces for           *)
 (* non-tail-recursive and tail-recursive merge functions, respectively.       *)
 Module Type MergeSig.
-Import MergeR.
 Parameter merge : forall (T : Type) (leT : rel T), seq T -> seq T -> seq T.
 Parameter mergeE : forall (T : Type) (leT : rel T), merge leT =2 path.merge leT.
-Parameter merge_R : merge_ty_R merge merge.
 End MergeSig.
 
 Module Type RevmergeSig.
-Import MergeR.
 Parameter revmerge : forall (T : Type) (leT : rel T), seq T -> seq T -> seq T.
 Parameter revmergeE : forall (T : Type) (leT : rel T) (xs ys : seq T),
     revmerge leT xs ys = rev (path.merge leT xs ys).
-Parameter revmerge_R : merge_ty_R revmerge revmerge.
 End RevmergeSig.
 
 (* The [Merge] module implements a non-tail-recursive merge function using    *)
@@ -180,8 +93,6 @@ Fixpoint merge (T : Type) (leT : rel T) (xs ys : seq T) : seq T :=
 
 Lemma mergeE (T : Type) (leT : rel T) : merge leT =2 path.merge leT.
 Proof. by elim=> // x xs IHxs; elim=> //= y ys IHys; rewrite IHxs IHys. Qed.
-
-Parametricity merge.
 
 End Merge.
 
@@ -201,12 +112,12 @@ Fixpoint wf_mergeord (T : Type) (xs ys : seq T) : Acc mergeord (xs, ys) :=
            (x :: xs', y :: ys')
            (fun _ H =>
               match H with
-                | or_introl H0 =>
-                  let: erefl in (_ = y1) := H0 return Acc mergeord y1 in
-                  wf_mergeord xs' (y :: ys')
-                | or_intror H0 =>
-                  let: erefl in (_ = y1) := H0 return Acc mergeord y1 in
-                  wf_mergeord' ys'
+              | or_introl H0 =>
+                let: erefl in (_ = y1) := H0 return Acc mergeord y1 in
+                wf_mergeord xs' (y :: ys')
+              | or_intror H0 =>
+                let: erefl in (_ = y1) := H0 return Acc mergeord y1 in
+                wf_mergeord' ys'
               end)
        else
          Acc_intro (x :: xs', [::]) (fun _ => False_ind _)) ys
@@ -216,22 +127,22 @@ Fixpoint wf_mergeord (T : Type) (xs ys : seq T) : Acc mergeord (xs, ys) :=
 Fixpoint merge_rec (T : Type) (leT : rel T)
                    (xs ys : seq T) (fuel : Acc mergeord (xs, ys)) : seq T :=
   match fuel, xs, ys return xs = _ -> ys = _ -> _ with
-    | _, [::], ys => fun _ _ => ys
-    | _, xs, [::] => fun _ _ => xs
-    | Acc_intro fuel, x :: xs', y :: ys' =>
-      fun (xsE : x :: xs' = xs) (ysE : y :: ys' = ys) =>
-      if leT x y then
-        x :: @merge_rec T leT xs' ys
-          (fuel _ match xsE in _ = xs0, ysE in _ = ys0
-                        return mergeord (xs', ys0) (xs0, ys0) with
-                    erefl, erefl => or_introl erefl
-                  end)
-      else
-        y :: @merge_rec T leT xs ys'
-          (fuel _ match xsE in _ = xs0, ysE in _ = ys0
-                        return mergeord (xs0, ys') (xs0, ys0) with
-                    erefl, erefl => or_intror erefl
-                  end)
+  | _, [::], ys => fun _ _ => ys
+  | _, xs, [::] => fun _ _ => xs
+  | Acc_intro fuel, x :: xs', y :: ys' =>
+    fun (xsE : x :: xs' = xs) (ysE : y :: ys' = ys) =>
+    if leT x y then
+      x :: @merge_rec T leT xs' ys
+        (fuel _ match xsE in _ = xs0, ysE in _ = ys0
+                      return mergeord (xs', ys0) (xs0, ys0) with
+                  erefl, erefl => or_introl erefl
+                end)
+    else
+      y :: @merge_rec T leT xs ys'
+        (fuel _ match xsE in _ = xs0, ysE in _ = ys0
+                      return mergeord (xs0, ys') (xs0, ys0) with
+                  erefl, erefl => or_intror erefl
+                end)
   end erefl erefl.
 
 Definition merge (T : Type) (leT : rel T) (xs ys : seq T) : seq T :=
@@ -242,10 +153,6 @@ Proof.
 rewrite /merge => xs ys; move: xs ys (wf_mergeord xs ys).
 by elim=> [|x xs IHxs]; elim=> [|y ys IHys] [acc] //=; rewrite IHxs IHys.
 Qed.
-
-Parametricity mergeord.
-Parametricity wf_mergeord.
-Parametricity merge.
 
 End MergeAcc.
 
@@ -275,8 +182,6 @@ elim: xs ys [::] => [|x xs IHxs]; elim=> [|y ys IHys] accu //=;
 by case: ifP => _; rewrite rev_cons cat_rcons.
 Qed.
 
-Parametricity revmerge.
-
 End Revmerge.
 
 (* The [RevmergeAcc] module implements a tail-recursive merge function using  *)
@@ -288,22 +193,22 @@ Import MergeAcc.
 Fixpoint merge_rec (T : Type) (leT : rel T) (xs ys accu : seq T)
                    (fuel : Acc mergeord (xs, ys)) : seq T :=
   match fuel, xs, ys return xs = _ -> ys = _ -> _ with
-    | _, [::], ys => fun _ _ => catrev ys accu
-    | _, xs, [::] => fun _ _ => catrev xs accu
-    | Acc_intro fuel, x :: xs', y :: ys' =>
-      fun (xsE : x :: xs' = xs) (ysE : y :: ys' = ys) =>
-      if leT x y then
-        @merge_rec T leT xs' ys (x :: accu)
-          (fuel _ match xsE in _ = xs0, ysE in _ = ys0
-                        return mergeord (xs', ys0) (xs0, ys0) with
-                    erefl, erefl => or_introl erefl
-                  end)
-      else
-        @merge_rec T leT xs ys' (y :: accu)
-          (fuel _ match xsE in _ = xs0, ysE in _ = ys0
-                        return mergeord (xs0, ys') (xs0, ys0) with
-                    erefl, erefl => or_intror erefl
-                  end)
+  | _, [::], ys => fun _ _ => catrev ys accu
+  | _, xs, [::] => fun _ _ => catrev xs accu
+  | Acc_intro fuel, x :: xs', y :: ys' =>
+    fun (xsE : x :: xs' = xs) (ysE : y :: ys' = ys) =>
+    if leT x y then
+      @merge_rec T leT xs' ys (x :: accu)
+        (fuel _ match xsE in _ = xs0, ysE in _ = ys0
+                      return mergeord (xs', ys0) (xs0, ys0) with
+                  erefl, erefl => or_introl erefl
+                end)
+    else
+      @merge_rec T leT xs ys' (y :: accu)
+        (fuel _ match xsE in _ = xs0, ysE in _ = ys0
+                      return mergeord (xs0, ys') (xs0, ys0) with
+                  erefl, erefl => or_intror erefl
+                end)
   end erefl erefl.
 
 Definition revmerge (T : Type) (leT : rel T) (xs ys : seq T) : seq T :=
@@ -318,8 +223,6 @@ elim=> [|x xs IHxs]; elim=> [|y ys IHys] accu [acc] //=;
 by case: ifP => _; rewrite rev_cons cat_rcons.
 Qed.
 
-Parametricity revmerge.
-
 End RevmergeAcc.
 
 (******************************************************************************)
@@ -327,25 +230,31 @@ End RevmergeAcc.
 (******************************************************************************)
 
 Module Insertion.
+
+Module Abstract.
+
+Definition sort (T R : Type) (leT : rel T)
+  (merge : R -> R -> R) (merge' : R -> R -> R)
+  (singleton : T -> R) (empty : R) :=
+  foldr (fun x => merge (singleton x)) empty.
+
+Parametricity sort.
+
+End Abstract.
+
 Section Insertion.
 
 Variables (T : Type) (leT : rel T).
 
-Definition sort := foldr (fun x => merge leT [:: x]) [::].
+Definition sort : seq T -> seq T := foldr (fun x => merge leT [:: x]) [::].
 
-Import StableSort.
-
-Lemma sortP : trace_sort leT sort.
-Proof.
-elim=> [|x _ [t -> /= ->]]; first by exists empty_trace.
-by exists (branch_trace true (leaf_trace true [:: x] erefl) t).
-Qed.
+Lemma asort_catE : Abstract.sort leT cat cat (fun x => [:: x]) [::] =1 id.
+Proof. by elim=> //= x xs ->. Qed.
 
 End Insertion.
 
-Parametricity sort.
-
-Definition sort_stable := StableSort.Pack sort sort_R sortP.
+Definition sort_stable :=
+  StableSort sort Abstract.sort Abstract.sort_R (fun _ _ _ => erefl) asort_catE.
 
 End Insertion.
 
@@ -375,195 +284,304 @@ Canonical Insertion.sort_stable.
 
 Module CBN_ (M : MergeSig).
 
-Section CBN.
+Module Abstract.
+Section Abstract.
 
-Variable (T : Type) (leT : rel T).
+Variables (T R : Type) (leT : rel T).
+Variables (merge : R -> R -> R) (merge' : R -> R -> R).
+Variables (singleton : T -> R) (empty : R).
 
-Let condrev (r : bool) (s : seq T) : seq T := if r then rev s else s.
-
-Fixpoint merge_sort_push (s : seq T) (stack : seq (seq T)) : seq (seq T) :=
+Fixpoint push (xs : R) (stack : seq (option R)) : seq (option R) :=
   match stack with
-  | [::] :: stack' | [::] as stack' => s :: stack'
-  | s' :: stack' => [::] :: merge_sort_push (M.merge leT s' s) stack'
+  | None :: stack | [::] as stack => Some xs :: stack
+  | Some ys :: stack => None :: push (merge ys xs) stack
   end.
 
-Fixpoint merge_sort_pop (s1 : seq T) (stack : seq (seq T)) : seq T :=
-  if stack is s2 :: stack' then
-    merge_sort_pop (M.merge leT s2 s1) stack' else s1.
-
-Fixpoint sort1rec (stack : seq (seq T)) (s : seq T) : seq T :=
-  if s is x :: s then sort1rec (merge_sort_push [:: x] stack) s else
-  merge_sort_pop [::] stack.
-
-Definition sort1 : seq T -> seq T := sort1rec [::].
-
-Fixpoint sort2rec (stack : seq (seq T)) (s : seq T) : seq T :=
-  if s is [:: x1, x2 & s'] then
-    let s1 := if leT x1 x2 then [:: x1; x2] else [:: x2; x1] in
-    sort2rec (merge_sort_push s1 stack) s'
-  else merge_sort_pop s stack.
-
-Definition sort2 : seq T -> seq T := sort2rec [::].
-
-Fixpoint sort3rec (stack : seq (seq T)) (s : seq T) : seq T :=
-  match s with
-    | [:: x1, x2, x3 & s'] =>
-      let s1 :=
-          if leT x1 x2 then
-            if leT x2 x3 then [:: x1; x2; x3]
-            else if leT x1 x3 then [:: x1; x3; x2] else [:: x3; x1; x2]
-          else
-            if leT x1 x3 then [:: x2; x1; x3]
-            else if leT x2 x3 then [:: x2; x3; x1] else [:: x3; x2; x1]
-      in
-      sort3rec (merge_sort_push s1 stack) s'
-    | [:: x1; x2] =>
-      merge_sort_pop (if leT x1 x2 then s else [:: x2; x1]) stack
-    | _ => merge_sort_pop s stack
+Fixpoint pop (xs : R) (stack : seq (option R)) : R :=
+  match stack with
+  | [::] => xs
+  | None :: stack => pop xs stack
+  | Some ys :: stack => pop (merge ys xs) stack
   end.
 
-Definition sort3 : seq T -> seq T := sort3rec [::].
-
-Fixpoint sortNrec (stack : seq (seq T)) (x : T) (s : seq T) : seq T :=
-  if s is y :: s then
-    if leT x y then incr stack y s [:: x] else decr stack y s [:: x]
+Fixpoint sort1rec (stack : seq (option R)) (xs : seq T) : R :=
+  if xs is x :: xs then
+    sort1rec (push (singleton x) stack) xs
   else
-    merge_sort_pop [:: x] stack
-with incr (stack : seq (seq T)) (x : T) (s accu : seq T) : seq T :=
-  if s is y :: s then
+    pop empty stack.
+
+#[using="All"]
+Definition sort1 : seq T -> R := sort1rec [::].
+
+Fixpoint sort2rec (stack : seq (option R)) (xs : seq T) : R :=
+  match xs with
+  | [:: x1, x2 & xs] =>
+    sort2rec (push (merge (singleton x1) (singleton x2)) stack) xs
+  | [:: x] => pop (singleton x) stack
+  | [::] => pop empty stack
+  end.
+
+#[using="All"]
+Definition sort2 : seq T -> R := sort2rec [::].
+
+Fixpoint sort3rec (stack : seq (option R)) (xs : seq T) : R :=
+  match xs with
+  | [:: x1, x2, x3 & xs] =>
+    let t := merge' (merge (singleton x1) (singleton x2)) (singleton x3) in
+    sort3rec (push t stack) xs
+  | [:: x1; x2] => pop (merge (singleton x1) (singleton x2)) stack
+  | [:: x] => pop (singleton x) stack
+  | [::] => pop empty stack
+  end.
+
+#[using="All"]
+Definition sort3 : seq T -> R := sort3rec [::].
+
+Fixpoint sortNrec (stack : seq (option R)) (x : T) (xs : seq T) : R :=
+  if xs is y :: xs then
     if leT x y then
-      incr stack y s (x :: accu)
+      incr stack y xs (singleton x)
     else
-      sortNrec (merge_sort_push (catrev accu [:: x]) stack) y s
+      decr stack y xs (singleton x)
   else
-    merge_sort_pop (catrev accu [:: x]) stack
-with decr (stack : seq (seq T)) (x : T) (s accu : seq T) : seq T :=
-  if s is y :: s then
+    pop (singleton x) stack
+with incr (stack : seq (option R)) (x : T) (xs : seq T) (accu : R) : R :=
+  if xs is y :: xs then
     if leT x y then
-      sortNrec (merge_sort_push (x :: accu) stack) y s
+      incr stack y xs (merge' accu (singleton x))
     else
-      decr stack y s (x :: accu)
+      sortNrec (push (merge' accu (singleton x)) stack) y xs
   else
-    merge_sort_pop (x :: accu) stack.
+    pop (merge' accu (singleton x)) stack
+with decr (stack : seq (option R)) (x : T) (xs : seq T) (accu : R) : R :=
+  if xs is y :: xs then
+    if leT x y then
+      sortNrec (push (merge accu (singleton x)) stack) y xs
+    else
+      decr stack y xs (merge accu (singleton x))
+  else
+    pop (merge accu (singleton x)) stack.
 
-Definition sortN (s : seq T) : seq T :=
-  if s is x :: s then sortNrec [::] x s else [::].
+#[using="All"]
+Definition sortN (xs : seq T) : R :=
+  if xs is x :: xs then sortNrec [::] x xs else empty.
 
-(* Proofs *)
+End Abstract.
 
-Import StableSort.
-
-Local Notation trace_sort := (trace_sort leT).
-Let flatten_stack := foldr (fun x => cat^~ (@flatten_trace _ leT x)) nil.
-
-Definition trace_sort_rec sort_rec := forall s stack, {t : trace leT |
-   flatten_stack stack ++ s = flatten_trace t &
-   sort_rec [seq sort_trace i | i <- stack] s = sort_trace t}.
-
-Lemma trace_sortP sort : trace_sort_rec sort -> trace_sort (sort [::]).
-Proof. by move/(_ _ [::]). Qed.
-
-Lemma merge_sort_pushP (t : trace leT) (stack : seq (trace leT)) :
-  {stack' : seq (trace leT) |
-    flatten_stack (t :: stack) = flatten_stack stack' &
-    merge_sort_push (sort_trace t) (map sort_trace stack) =
-    map sort_trace stack'}.
-Proof.
-elim: stack t => [|t' stack IHstack] t /=; first by exists [:: t].
-rewrite M.mergeE ifnilE -catA; case: trace_nilP => _ _.
-  by exists (t :: stack); rewrite //= cats0.
-have [/= {IHstack}stack -> ->] := IHstack (branch_trace true t' t).
-by exists (empty_trace :: stack); rewrite //= cats0.
-Qed.
-
-Lemma merge_sort_popP (t : trace leT) (stack : seq (trace leT)) :
-  {t' : trace leT |
-    flatten_stack (t :: stack) = flatten_trace t' &
-    merge_sort_pop (sort_trace t) (map sort_trace stack) = sort_trace t'}.
-Proof.
-elim: stack t => [|t' stack IHstack] t; first by exists t; rewrite //= cats0.
-rewrite /= M.mergeE -catA.
-by have [/= t'' -> ->] := IHstack (branch_trace true t' t); exists t''.
-Qed.
-
-Lemma sort1P : trace_sort sort1.
-Proof.
-apply/trace_sortP; elim=> [|x s IHs] stack; first exact: merge_sort_popP [tr] _.
-case: (merge_sort_pushP [tr<= x] stack).
-by rewrite (catA _ [:: _]) => {}stack /= -> ->; exact: IHs.
-Qed.
-
-Lemma sort2P : trace_sort sort2.
-Proof.
-apply/trace_sortP => s; have [n] := ubnP (size s); elim: n s => // n IHn.
-move=> [|x [|y s]]/=; rewrite ?ltnS => size_s stack.
-- exact: merge_sort_popP [tr<=] _.
-- exact: merge_sort_popP [tr<= x] _.
-case: (merge_sort_pushP [tr x; y] stack).
-by rewrite (catA _ [:: _; _]) => /= {}stack -> ->; apply/IHn/ltnW.
-Qed.
-
-Lemma sort3P : trace_sort sort3.
-Proof.
-apply/trace_sortP => s; have [n] := ubnP (size s); elim: n s => // n IHn.
-move=> [|x [|y [|z s]]]/=; rewrite ?ltnS => size_s stack.
-- exact: merge_sort_popP [tr<=] _.
-- exact: merge_sort_popP [tr<= x] _.
-- exact: merge_sort_popP [tr x; y] _.
-rewrite (catA _ [:: _; _; _]).
-pose xyz : trace leT := branch_trace false [tr x; y] [tr<= z].
-case: (merge_sort_pushP xyz stack) => /= stack' ->.
-set push1 := merge_sort_push _ _; set push2 := merge_sort_push _ _.
-have ->: push1 = push2 by congr merge_sort_push; do 3 case: ifP => //=.
-by move=> ->; apply/IHn/ltnW/ltnW.
-Qed.
-
-Lemma sortNP : trace_sort sortN.
-Proof.
-case=> /= [|x s]; first by exists empty_trace.
-suff /(_ [::]) : forall stack, {t : trace leT |
-   flatten_stack stack ++ x :: s = flatten_trace t &
-   sortNrec [seq sort_trace i | i <- stack] x s = sort_trace t} by [].
-have [n] := ubnP (size s); elim: n x s => // n IHn x [|y s]/= sn stack.
-  exact: merge_sort_popP [tr<= x] _.
-set lexy := leT x y.
-have: path (fun y x => leT x y == lexy) y [:: x] by rewrite /= eqxx.
-have ->: [:: x, y & s] = rev [:: y; x] ++ s by [].
-elim: s sn (lexy) (y) [:: x] => {lexy x y} => [|y s IHs' /=] /ltnW sn ord x acc.
-  rewrite -/(sorted _ (_ :: _)) -rev_sorted cats0 => sorted_acc.
-  case: (merge_sort_popP (leaf_trace ord _ sorted_acc) stack) => /= t ->.
-  by rewrite revK; case: ord {sorted_acc} => ->; exists t.
-case: ord (boolP (leT x y)) => [] [] lexy.
-- move=> path_acc.
-  have: path (fun y x => leT x y == true) y (x :: acc) by rewrite /= lexy eqxx.
-  by move=> /(IHs' sn)[t]; rewrite -cat_rcons -rev_cons => -> ->; exists t.
-- rewrite -/(sorted _ (_ :: _)) -rev_sorted => sorted_acc.
-  case: (merge_sort_pushP (leaf_trace true _ sorted_acc) stack) => stack'.
-  by rewrite /= catA => -> ->; apply/IHn.
-- rewrite -/(sorted _ (_ :: _)) -rev_sorted => sorted_acc.
-  case: (merge_sort_pushP (leaf_trace false _ sorted_acc) stack) => stack'.
-  by rewrite /= catA revK => -> ->; apply/IHn.
-- move=> path_acc.
-  have: path (fun y x => leT x y == false) y (x :: acc).
-    by rewrite /= eqbF_neg lexy.
-  by move=> /(IHs' sn)[t]; rewrite -cat_rcons -rev_cons => -> ->; exists t.
-Qed.
-
-End CBN.
-
-Realizer M.merge as merge_R arity 2 := M.merge_R.
-
-Parametricity merge_sort_push.
-Parametricity merge_sort_pop.
 Parametricity sort1.
 Parametricity sort2.
 Parametricity sort3.
 Parametricity sortN.
 
-Definition sort1_stable := StableSort.Pack sort1 sort1_R sort1P.
-Definition sort2_stable := StableSort.Pack sort2 sort2_R sort2P.
-Definition sort3_stable := StableSort.Pack sort3 sort3_R sort3P.
-Definition sortN_stable := StableSort.Pack sortN sortN_R sortNP.
+End Abstract.
+
+Section CBN.
+
+Variable (T : Type) (leT : rel T).
+
+Fixpoint push (xs : seq T) (stack : seq (seq T)) : seq (seq T) :=
+  match stack with
+  | [::] :: stack | [::] as stack => xs :: stack
+  | ys :: stack => [::] :: push (M.merge leT ys xs) stack
+  end.
+
+Fixpoint pop (xs : seq T) (stack : seq (seq T)) : seq T :=
+  if stack is ys :: stack then pop (M.merge leT ys xs) stack else xs.
+
+Fixpoint sort1rec (stack : seq (seq T)) (xs : seq T) : seq T :=
+  if xs is x :: xs then sort1rec (push [:: x] stack) xs else pop [::] stack.
+
+Definition sort1 : seq T -> seq T := sort1rec [::].
+
+Fixpoint sort2rec (stack : seq (seq T)) (xs : seq T) : seq T :=
+  if xs is [:: x1, x2 & xs] then
+    let t := if leT x1 x2 then [:: x1; x2] else [:: x2; x1] in
+    sort2rec (push t stack) xs
+  else pop xs stack.
+
+Definition sort2 : seq T -> seq T := sort2rec [::].
+
+Fixpoint sort3rec (stack : seq (seq T)) (xs : seq T) : seq T :=
+  match xs with
+  | [:: x1, x2, x3 & xs] =>
+    let t :=
+        if leT x1 x2 then
+          if leT x2 x3 then [:: x1; x2; x3]
+          else if leT x1 x3 then [:: x1; x3; x2] else [:: x3; x1; x2]
+        else
+          if leT x1 x3 then [:: x2; x1; x3]
+          else if leT x2 x3 then [:: x2; x3; x1] else [:: x3; x2; x1]
+    in
+    sort3rec (push t stack) xs
+  | [:: x1; x2] => pop (if leT x1 x2 then xs else [:: x2; x1]) stack
+  | _ => pop xs stack
+  end.
+
+Definition sort3 : seq T -> seq T := sort3rec [::].
+
+Fixpoint sortNrec (stack : seq (seq T)) (x : T) (xs : seq T) : seq T :=
+  if xs is y :: xs then
+    if leT x y then incr stack y xs [:: x] else decr stack y xs [:: x]
+  else
+    pop [:: x] stack
+with incr (stack : seq (seq T)) (x : T) (xs accu : seq T) : seq T :=
+  if xs is y :: xs then
+    if leT x y then
+      incr stack y xs (x :: accu)
+    else
+      sortNrec (push (catrev accu [:: x]) stack) y xs
+  else
+    pop (catrev accu [:: x]) stack
+with decr (stack : seq (seq T)) (x : T) (xs accu : seq T) : seq T :=
+  if xs is y :: xs then
+    if leT x y then
+      sortNrec (push (x :: accu) stack) y xs
+    else
+      decr stack y xs (x :: accu)
+  else
+    pop (x :: accu) stack.
+
+Definition sortN (xs : seq T) : seq T :=
+  if xs is x :: xs then sortNrec [::] x xs else [::].
+
+(* Proofs *)
+
+Let geT x y := leT y x.
+Let astack_of_stack : seq (seq T) -> seq (option (seq T)) :=
+  map (fun xs => if xs is [::] then None else Some xs).
+
+Notation merge := (path.merge leT) (only parsing).
+Notation merge' :=
+  (fun xs ys => rev (path.merge geT (rev ys) (rev xs))) (only parsing).
+Notation flatten_stack :=
+  (foldl (fun xs : seq T => oapp (cat^~ xs) xs)) (only parsing).
+
+Lemma apop_mergeE xs stack :
+  Abstract.pop merge xs (astack_of_stack stack) = pop xs stack.
+Proof.
+by elim: stack xs => [|[|y ys] stack IHstack] xs //=; rewrite M.mergeE IHstack.
+Qed.
+
+Lemma apush_mergeE xs stack :
+  ~~ nilp xs ->
+  Abstract.push merge xs (astack_of_stack stack)
+  = astack_of_stack (push xs stack).
+Proof.
+elim: stack xs => [|[|y ys] stack IHstack]; try by case.
+by move=> xs Hxs /=; rewrite M.mergeE IHstack // /nilp size_merge.
+Qed.
+
+Lemma asort1_mergeE :
+  Abstract.sort1 leT merge merge' (fun x => [:: x]) [::] =1 sort1.
+Proof.
+rewrite /Abstract.sort1 /sort1 -[Nil (option _)]/(astack_of_stack [::]) => xs.
+elim: xs (Nil (seq _)) => /= [|x xs IHxs] stack; first by rewrite apop_mergeE.
+by rewrite -IHxs apush_mergeE.
+Qed.
+
+Lemma asort2_mergeE :
+  Abstract.sort2 leT merge merge' (fun x => [:: x]) [::] =1 sort2.
+Proof.
+move=> xs; have [n] := ubnP (size xs).
+rewrite /Abstract.sort2 /sort2 -[Nil (option _)]/(astack_of_stack [::]).
+elim: n (Nil (seq _)) xs => // n IHn stack [|x [|x' xs /= /ltnW /IHn <-]] /=;
+  try by rewrite apop_mergeE.
+by rewrite apush_mergeE; last case: ifP.
+Qed.
+
+Lemma asort3_mergeE :
+  Abstract.sort3 leT merge merge' (fun x => [:: x]) [::] =1 sort3.
+Proof.
+move=> xs; have [n] := ubnP (size xs).
+rewrite /Abstract.sort3 /sort3 -[Nil (option _)]/(astack_of_stack [::]).
+move: n (Nil (seq _)) xs.
+elim=> // n IHn stack [|x [|x' [|x'' xs /= /ltnW /ltnW /IHn <-]]] /=;
+  try by rewrite apop_mergeE.
+rewrite apush_mergeE; last by rewrite /nilp !(size_rev, size_merge).
+by rewrite !(fun_if rev, fun_if (path.merge _ _), fun_if (cons _)).
+Qed.
+
+Lemma asortN_mergeE :
+  Abstract.sortN leT merge merge' (fun x => [:: x]) [::] =1 sortN.
+Proof.
+case=> // x xs; have [n] := ubnP (size xs).
+rewrite /Abstract.sortN /sortN -[Nil (option _)]/(astack_of_stack [::]).
+elim: n (Nil (seq _)) x xs => // n IHn stack x [|y xs /= /ltnSE Hxs].
+  by rewrite [LHS]apop_mergeE.
+rewrite /Abstract.sortNrec.
+rewrite -/(Abstract.incr _ _ merge' _) -/(Abstract.decr _ _ merge' _).
+pose rs := Nil T; rewrite -{1}[[:: x]]/(rcons (rev rs) x) -/(x :: rs).
+elim: xs Hxs x y rs => [_|z xs IHxs /= /ltnW Hxs] x y rs.
+  rewrite /Abstract.incr /Abstract.decr !apop_mergeE rev_rcons revK /= /geT.
+  by case: leT.
+rewrite /Abstract.incr -/(Abstract.incr _ _ merge' _).
+rewrite /Abstract.decr -/(Abstract.decr _ _ merge' _).
+rewrite -/(Abstract.sortNrec _ _ merge' _).
+move: (IHxs Hxs y z (x :: rs)); rewrite -rev_cons rev_rcons revK /= /geT.
+by do 2 case: leT; rewrite // apush_mergeE ?rev_nilp // IHn.
+Qed.
+
+Lemma apush_catE (xs ys : seq T) stack :
+  flatten_stack ys (Abstract.push cat xs stack)
+  = flatten_stack (xs ++ ys) stack.
+Proof.
+by elim: stack xs => [|[zs|] stack IHstack] xs //=; rewrite IHstack catA.
+Qed.
+
+Lemma apop_catE xs stack : Abstract.pop cat xs stack = flatten_stack xs stack.
+Proof. by elim: stack xs => [|[]] /=. Qed.
+
+Lemma asort1_catE : Abstract.sort1 leT cat cat (fun x => [:: x]) [::] =1 id.
+Proof.
+move=> xs; rewrite /Abstract.sort1 -[RHS]/(flatten_stack xs [::]).
+elim: xs (Nil (option _)) => /= [|x xs IHxs] stack; first exact: apop_catE.
+by rewrite IHxs apush_catE.
+Qed.
+
+Lemma asort2_catE : Abstract.sort2 leT cat cat (fun x => [:: x]) [::] =1 id.
+Proof.
+move=> xs; have [n] := ubnP (size xs).
+rewrite /Abstract.sort2 -[RHS]/(flatten_stack xs [::]).
+move: n (Nil (option _)) xs.
+by elim=> // n IHn stack [|x [|x' xs /= /ltnW /IHn ->]] /=;
+  rewrite (apop_catE, apush_catE).
+Qed.
+
+Lemma asort3_catE : Abstract.sort3 leT cat cat (fun x => [:: x]) [::] =1 id.
+Proof.
+move=> xs; have [n] := ubnP (size xs).
+rewrite /Abstract.sort3 -[RHS]/(flatten_stack xs [::]).
+move: n (Nil (option _)) xs.
+by elim=> // n IHn stack [|x [|x' [|x'' xs /= /ltnW /ltnW /IHn ->]]] /=;
+  rewrite (apop_catE, apush_catE).
+Qed.
+
+Lemma asortN_catE : Abstract.sortN leT cat cat (fun x => [:: x]) [::] =1 id.
+Proof.
+case=> // x xs; have [n] := ubnP (size xs).
+rewrite /Abstract.sortN -[RHS]/(flatten_stack (x :: xs) [::]).
+elim: n x (Nil (option _)) xs => // n IHn x stack [|y xs /= /ltnSE Hxs];
+  first by rewrite [LHS]apop_catE.
+rewrite /Abstract.sortNrec -/(Abstract.incr _ _ _ _) -/(Abstract.decr _ _ _ _).
+pose rs := Nil T; rewrite -[x :: y :: _]/(rs ++ _) -[[:: x]]/(rs ++ _).
+elim: xs Hxs x y rs => [_|z xs IHxs /= /ltnW Hxs] x y rs.
+  by rewrite if_same [LHS]apop_catE -catA.
+rewrite /Abstract.incr -/(Abstract.incr _ _ _ _).
+rewrite /Abstract.decr -/(Abstract.decr _ _ _ _) -/(Abstract.sortNrec _ _ _ _).
+move: (IHxs Hxs y z (rcons rs x)); rewrite IHn // apush_catE -cats1 -!catA /=.
+by case: leT => ->; rewrite if_same.
+Qed.
+
+End CBN.
+
+Definition sort1_stable :=
+  StableSort sort1 Abstract.sort1 Abstract.sort1_R asort1_mergeE asort1_catE.
+Definition sort2_stable :=
+  StableSort sort2 Abstract.sort2 Abstract.sort2_R asort2_mergeE asort2_catE.
+Definition sort3_stable :=
+  StableSort sort3 Abstract.sort3 Abstract.sort3_R asort3_mergeE asort3_catE.
+Definition sortN_stable :=
+  StableSort sortN Abstract.sortN Abstract.sortN_R asortN_mergeE asortN_catE.
 
 End CBN_.
 
@@ -599,231 +617,346 @@ Canonical CBNAcc.sortN_stable.
 (******************************************************************************)
 
 Module CBV_ (M : RevmergeSig).
-Section CBV.
 
-Variables (T : Type) (leT : rel T).
-Let geT x y := leT y x.
+Module Abstract.
+Section Abstract.
 
-Let condrev (r : bool) (s : seq T) : seq T := if r then rev s else s.
+Variables (T R : Type) (leT : rel T).
+Variables (merge : R -> R -> R) (merge' : R -> R -> R).
+Variables (singleton : T -> R) (empty : R).
 
-Fixpoint merge_sort_push (xs : seq T) (stack : seq (seq T)) : seq (seq T) :=
+Fixpoint push (xs : R) (stack : seq (option R)) : seq (option R) :=
   match stack with
-    | [::] :: stack' | [::] as stack' => xs :: stack'
-    | ys :: [::] :: stack | ys :: ([::] as stack) =>
-      [::] :: M.revmerge leT ys xs :: stack
-    | ys :: zs :: stack =>
-      [::] :: [::] ::
-           merge_sort_push (M.revmerge geT (M.revmerge leT ys xs) zs) stack
+  | None :: stack | [::] as stack => Some xs :: stack
+  | Some ys :: None :: stack | Some ys :: ([::] as stack) =>
+    None :: Some (merge ys xs) :: stack
+  | Some ys :: Some zs :: stack =>
+    None :: None :: push (merge' zs (merge ys xs)) stack
   end.
 
-Fixpoint merge_sort_pop
-         (mode : bool) (xs : seq T) (stack : seq (seq T)) : seq T :=
-  match stack, mode with
-    | [::], true => rev xs
-    | [::], false => xs
-    | [::] :: [::] :: stack, _ => merge_sort_pop mode xs stack
-    | [::] :: stack, _ => merge_sort_pop (~~ mode) (rev xs) stack
-    | ys :: stack, true => merge_sort_pop false (M.revmerge geT xs ys) stack
-    | ys :: stack, false => merge_sort_pop true (M.revmerge leT ys xs) stack
+Fixpoint pop (mode : bool) (xs : R) (stack : seq (option R)) : R :=
+  match stack with
+  | [::] => xs
+  | None :: None :: stack => pop mode xs stack
+  | None :: stack => pop (~~ mode) xs stack
+  | (Some ys) :: stack =>
+    pop (~~ mode) (if mode then merge' ys xs else merge ys xs) stack
   end.
 
-Fixpoint sort1rec (stack : seq (seq T)) (s : seq T) : seq T :=
-  if s is x :: s then sort1rec (merge_sort_push [:: x] stack) s else
-  merge_sort_pop false [::] stack.
-
-Definition sort1 : seq T -> seq T := sort1rec [::].
-
-Fixpoint sort2rec (stack : seq (seq T)) (s : seq T) : seq T :=
-  if s is [:: x1, x2 & s'] then
-    let s1 := if leT x1 x2 then [:: x1; x2] else [:: x2; x1] in
-    sort2rec (merge_sort_push s1 stack) s'
-  else merge_sort_pop false s stack.
-
-Definition sort2 : seq T -> seq T := sort2rec [::].
-
-Fixpoint sort3rec (stack : seq (seq T)) (s : seq T) : seq T :=
-  match s with
-    | [:: x1, x2, x3 & s'] =>
-      let s1 :=
-          if leT x1 x2 then
-            if leT x2 x3 then [:: x1; x2; x3]
-            else if leT x1 x3 then [:: x1; x3; x2] else [:: x3; x1; x2]
-          else
-            if leT x1 x3 then [:: x2; x1; x3]
-            else if leT x2 x3 then [:: x2; x3; x1] else [:: x3; x2; x1]
-      in
-      sort3rec (merge_sort_push s1 stack) s'
-    | [:: x1; x2] =>
-      merge_sort_pop false (if leT x1 x2 then s else [:: x2; x1]) stack
-    | _ => merge_sort_pop false s stack
-  end.
-
-Definition sort3 : seq T -> seq T := sort3rec [::].
-
-Fixpoint sortNrec (stack : seq (seq T)) (x : T) (s : seq T) : seq T :=
-  if s is y :: s then
-    if leT x y then incr stack y s [:: x] else decr stack y s [:: x]
+Fixpoint sort1rec (stack : seq (option R)) (xs : seq T) : R :=
+  if xs is x :: xs then
+    sort1rec (push (singleton x) stack) xs
   else
-    merge_sort_pop false [:: x] stack
-with incr (stack : seq (seq T)) (x : T) (s accu : seq T) : seq T :=
-  if s is y :: s then
+    pop false empty stack.
+
+#[using="All"]
+Definition sort1 : seq T -> R := sort1rec [::].
+
+Fixpoint sort2rec (stack : seq (option R)) (xs : seq T) : R :=
+  match xs with
+  | [:: x1, x2 & xs] =>
+    sort2rec (push (merge (singleton x1) (singleton x2)) stack) xs
+  | [:: x] => pop false (singleton x) stack
+  | [::] => pop false empty stack
+  end.
+
+#[using="All"]
+Definition sort2 : seq T -> R := sort2rec [::].
+
+Fixpoint sort3rec (stack : seq (option R)) (xs : seq T) : R :=
+  match xs with
+  | [:: x1, x2, x3 & xs] =>
+    let t := merge' (merge (singleton x1) (singleton x2)) (singleton x3) in
+    sort3rec (push t stack) xs
+  | [:: x1; x2] => pop false (merge (singleton x1) (singleton x2)) stack
+  | [:: x] => pop false (singleton x) stack
+  | [::] => pop false empty stack
+  end.
+
+#[using="All"]
+Definition sort3 : seq T -> R := sort3rec [::].
+
+Fixpoint sortNrec (stack : seq (option R)) (x : T) (xs : seq T) : R :=
+  if xs is y :: xs then
     if leT x y then
-      incr stack y s (x :: accu)
+      incr stack y xs (singleton x)
     else
-      sortNrec (merge_sort_push (catrev accu [:: x]) stack) y s
+      decr stack y xs (singleton x)
   else
-    merge_sort_pop false (catrev accu [:: x]) stack
-with decr (stack : seq (seq T)) (x : T) (s accu : seq T) : seq T :=
-  if s is y :: s then
+    pop false (singleton x) stack
+with incr (stack : seq (option R)) (x : T) (xs : seq T) (accu : R) : R :=
+  if xs is y :: xs then
     if leT x y then
-      sortNrec (merge_sort_push (x :: accu) stack) y s
+      incr stack y xs (merge' accu (singleton x))
     else
-      decr stack y s (x :: accu)
+      sortNrec (push (merge' accu (singleton x)) stack) y xs
   else
-    merge_sort_pop false (x :: accu) stack.
+    pop false (merge' accu (singleton x)) stack
+with decr (stack : seq (option R)) (x : T) (xs : seq T) (accu : R) : R :=
+  if xs is y :: xs then
+    if leT x y then
+      sortNrec (push (merge accu (singleton x)) stack) y xs
+    else
+      decr stack y xs (merge accu (singleton x))
+  else
+    pop false (merge accu (singleton x)) stack.
 
-Definition sortN (s : seq T) : seq T :=
-  if s is x :: s then sortNrec [::] x s else [::].
+#[using="All"]
+Definition sortN (xs : seq T) : R :=
+  if xs is x :: xs then sortNrec [::] x xs else empty.
 
-(* Proofs *)
+End Abstract.
 
-Import StableSort.
-
-Local Notation trace_sort := (trace_sort leT).
-Let flatten_stack := foldr (fun x => cat^~ (@flatten_trace _ leT x)) nil.
-
-Let Fixpoint sort_stack (mode : bool) (stack : seq (trace leT)) : seq (seq T) :=
-  if stack isn't t :: stack then [::] else
-    condrev mode (sort_trace t) :: sort_stack (~~ mode) stack.
-
-Definition trace_sort_rec sort_rec := forall s stack, {t : trace leT |
-   flatten_stack stack ++ s = flatten_trace t &
-   sort_rec (sort_stack false stack) s = sort_trace t}.
-
-Lemma trace_sortP sort : trace_sort_rec sort -> trace_sort (sort [::]).
-Proof. by move/(_ _ [::]). Qed.
-
-Lemma merge_sort_pushP (t : trace leT) (stack : seq (trace leT)) :
-  {stack' : seq (trace leT) |
-    flatten_stack (t :: stack) = flatten_stack stack' &
-    merge_sort_push (sort_trace t) (sort_stack false stack)
-    = sort_stack false stack'}.
-Proof.
-move: t stack; fix IHstack 2; move=> t [|t' [|t'' stack]] /=.
-- by exists [:: t].
-- rewrite !M.revmergeE ifnilE trace_nilp; have [->|_] := nilP.
-    by exists [:: t].
-  by exists [:: empty_trace; branch_trace true t' t]; rewrite //= cats0.
-- rewrite !M.revmergeE !ifnilE rev_nilp !trace_nilp; have [->|_] := nilP.
-    by exists [:: t, t'' & stack]; rewrite ?cats0.
-  rewrite -!catA; have [->|_] := nilP.
-    exists [:: empty_trace, branch_trace true t' t & stack] => //.
-    by rewrite /= ?cats0.
-  have [/= {}stack -> ->] :=
-    IHstack (branch_trace false t'' (branch_trace true t' t)) stack.
-  by exists [:: empty_trace, empty_trace & stack]; rewrite /= ?cats0.
-Qed.
-
-Let nilp_condrev (r : bool) (s : seq T) : nilp (condrev r s) = nilp s.
-Proof. by case: r; rewrite ?rev_nilp. Qed.
-
-Lemma merge_sort_popP (mode : bool) (t : trace leT) (stack : seq (trace leT)) :
-  {t' : trace leT |
-    flatten_stack (t :: stack) = flatten_trace t' &
-    merge_sort_pop mode (condrev mode (sort_trace t)) (sort_stack mode stack)
-    = sort_trace t'}.
-Proof.
-move: mode t stack; fix IHstack 3; move=> mode t [|t' stack] /=.
-  by exists t => //; case: mode; rewrite ?revK.
-rewrite -catA !M.revmergeE ifnilE nilp_condrev.
-case: trace_nilP => _ _; last first.
-  by case: mode (IHstack (~~ mode) (branch_trace (~~ mode) t' t) stack).
-case: stack => [|t'' stack] /=.
-  by exists t => //; case: mode; rewrite ?revK.
-rewrite !M.revmergeE !ifnilE !nilp_condrev !negbK revK.
-case: trace_nilP => _ _; first by rewrite cats0; apply: IHstack.
-rewrite -catA.
-by case: mode (IHstack mode (branch_trace mode t'' t) stack); rewrite //= revK.
-Qed.
-
-Lemma sort1P : trace_sort sort1.
-Proof.
-apply/trace_sortP; elim=> [|x s IHs] stack; first exact: merge_sort_popP [tr] _.
-case: (merge_sort_pushP [tr<= x] stack).
-by rewrite (catA _ [:: _]) => {}stack /= -> ->; exact: IHs.
-Qed.
-
-Lemma sort2P : trace_sort sort2.
-Proof.
-apply/trace_sortP => s; have [n] := ubnP (size s); elim: n s => // n IHn.
-move=> [|x [|y s]]/=; rewrite ?ltnS => size_s stack.
-- exact: merge_sort_popP [tr<=] _.
-- exact: merge_sort_popP [tr<= x] _.
-case: (merge_sort_pushP [tr x; y] stack).
-by rewrite (catA _ [:: _; _]) => /= {}stack -> ->; apply/IHn/ltnW.
-Qed.
-
-Lemma sort3P : trace_sort sort3.
-Proof.
-apply/trace_sortP => s; have [n] := ubnP (size s); elim: n s => // n IHn.
-move=> [|x [|y [|z s]]]/=; rewrite ?ltnS => size_s stack.
-- exact: merge_sort_popP [tr<=] _.
-- exact: merge_sort_popP [tr<= x] _.
-- exact: merge_sort_popP [tr x; y] _.
-rewrite (catA _ [:: _; _; _]).
-pose xyz : trace leT := branch_trace false [tr x; y] [tr<= z].
-case: (merge_sort_pushP xyz stack) => /= stack' ->.
-set push1 := merge_sort_push _ _; set push2 := merge_sort_push _ _.
-have ->: push1 = push2 by congr merge_sort_push; do 3 case: ifP => //=.
-by move=> ->; apply/IHn/ltnW/ltnW.
-Qed.
-
-Lemma sortNP : trace_sort sortN.
-Proof.
-case=> /= [|x s]; first by exists empty_trace.
-suff /(_ [::]) : forall stack, {t : trace leT |
-   flatten_stack stack ++ x :: s = flatten_trace t &
-   sortNrec (sort_stack false stack) x s = sort_trace t} by [].
-have [n] := ubnP (size s); elim: n x s => // n IHn x [|y s]/= sn stack.
-  exact: merge_sort_popP [tr<= x] _.
-set lexy := leT x y.
-have: path (fun y x => leT x y == lexy) y [:: x] by rewrite /= eqxx.
-have ->: [:: x, y & s] = rev [:: y; x] ++ s by [].
-elim: s sn (lexy) (y) [:: x] => {lexy x y} => [|y s IHs' /=] /ltnW sn ord x acc.
-  rewrite -/(sorted _ (_ :: _)) -rev_sorted cats0 => sorted_acc.
-  case: (merge_sort_popP false (leaf_trace ord _ sorted_acc) stack) => /= t ->.
-  by rewrite revK; case: ord {sorted_acc} => ->; exists t.
-case: ord (boolP (leT x y)) => [] [] lexy.
-- move=> path_acc.
-  have: path (fun y x => leT x y == true) y (x :: acc) by rewrite /= lexy eqxx.
-  by move=> /(IHs' sn)[t]; rewrite -cat_rcons -rev_cons => -> ->; exists t.
-- rewrite -/(sorted _ (_ :: _)) -rev_sorted => sorted_acc.
-  case: (merge_sort_pushP (leaf_trace true _ sorted_acc) stack) => stack'.
-  by rewrite /= catA => -> ->; apply/IHn.
-- rewrite -/(sorted _ (_ :: _)) -rev_sorted => sorted_acc.
-  case: (merge_sort_pushP (leaf_trace false _ sorted_acc) stack) => stack'.
-  by rewrite /= catA revK => -> ->; apply/IHn.
-- move=> path_acc.
-  have: path (fun y x => leT x y == false) y (x :: acc).
-    by rewrite /= eqbF_neg lexy.
-  by move=> /(IHs' sn)[t]; rewrite -cat_rcons -rev_cons => -> ->; exists t.
-Qed.
-
-End CBV.
-
-Realizer M.revmerge as revmerge_R arity 2 := M.revmerge_R.
-
-Parametricity merge_sort_push.
-Parametricity merge_sort_pop.
 Parametricity sort1.
 Parametricity sort2.
 Parametricity sort3.
 Parametricity sortN.
 
-Definition sort1_stable := StableSort.Pack sort1 sort1_R sort1P.
-Definition sort2_stable := StableSort.Pack sort2 sort2_R sort2P.
-Definition sort3_stable := StableSort.Pack sort3 sort3_R sort3P.
-Definition sortN_stable := StableSort.Pack sortN sortN_R sortNP.
+End Abstract.
+
+Section CBV.
+
+Variables (T : Type) (leT : rel T).
+Let geT x y := leT y x.
+
+Fixpoint push (xs : seq T) (stack : seq (seq T)) : seq (seq T) :=
+  match stack with
+  | [::] :: stack | [::] as stack => xs :: stack
+  | ys :: [::] :: stack | ys :: ([::] as stack) =>
+    [::] :: M.revmerge leT ys xs :: stack
+  | ys :: zs :: stack =>
+    [::] :: [::] :: push (M.revmerge geT (M.revmerge leT ys xs) zs) stack
+  end.
+
+Fixpoint pop (mode : bool) (xs : seq T) (stack : seq (seq T)) : seq T :=
+  match stack, mode with
+  | [::], true => rev xs
+  | [::], false => xs
+  | [::] :: [::] :: stack, _ => pop mode xs stack
+  | [::] :: stack, _ => pop (~~ mode) (rev xs) stack
+  | ys :: stack, true => pop false (M.revmerge geT xs ys) stack
+  | ys :: stack, false => pop true (M.revmerge leT ys xs) stack
+  end.
+
+Fixpoint sort1rec (stack : seq (seq T)) (xs : seq T) : seq T :=
+  if xs is x :: xs then
+    sort1rec (push [:: x] stack) xs
+  else
+    pop false [::] stack.
+
+Definition sort1 : seq T -> seq T := sort1rec [::].
+
+Fixpoint sort2rec (stack : seq (seq T)) (xs : seq T) : seq T :=
+  if xs is [:: x1, x2 & xs] then
+    let t := if leT x1 x2 then [:: x1; x2] else [:: x2; x1] in
+    sort2rec (push t stack) xs
+  else pop false xs stack.
+
+Definition sort2 : seq T -> seq T := sort2rec [::].
+
+Fixpoint sort3rec (stack : seq (seq T)) (xs : seq T) : seq T :=
+  match xs with
+  | [:: x1, x2, x3 & xs] =>
+    let t :=
+        if leT x1 x2 then
+          if leT x2 x3 then [:: x1; x2; x3]
+          else if leT x1 x3 then [:: x1; x3; x2] else [:: x3; x1; x2]
+        else
+          if leT x1 x3 then [:: x2; x1; x3]
+          else if leT x2 x3 then [:: x2; x3; x1] else [:: x3; x2; x1]
+    in
+    sort3rec (push t stack) xs
+  | [:: x1; x2] => pop false (if leT x1 x2 then xs else [:: x2; x1]) stack
+  | _ => pop false xs stack
+  end.
+
+Definition sort3 : seq T -> seq T := sort3rec [::].
+
+Fixpoint sortNrec (stack : seq (seq T)) (x : T) (xs : seq T) : seq T :=
+  if xs is y :: xs then
+    if leT x y then incr stack y xs [:: x] else decr stack y xs [:: x]
+  else
+    pop false [:: x] stack
+with incr (stack : seq (seq T)) (x : T) (xs accu : seq T) : seq T :=
+  if xs is y :: xs then
+    if leT x y then
+      incr stack y xs (x :: accu)
+    else
+      sortNrec (push (catrev accu [:: x]) stack) y xs
+  else
+    pop false (catrev accu [:: x]) stack
+with decr (stack : seq (seq T)) (x : T) (xs accu : seq T) : seq T :=
+  if xs is y :: xs then
+    if leT x y then
+      sortNrec (push (x :: accu) stack) y xs
+    else
+      decr stack y xs (x :: accu)
+  else
+    pop false (x :: accu) stack.
+
+Definition sortN (xs : seq T) : seq T :=
+  if xs is x :: xs then sortNrec [::] x xs else [::].
+
+(* Proofs *)
+
+Let condrev (r : bool) (s : seq T) : seq T := if r then rev s else s.
+
+Lemma condrev_nilp mode xs : nilp (condrev mode xs) = nilp xs.
+Proof. by case: mode; rewrite /= ?rev_nilp. Qed.
+
+Lemma condrevK mode : involutive (condrev mode).
+Proof. by case: mode; first exact: revK. Qed.
+
+Let Fixpoint astack_of_stack (mode : bool) (stack : seq (seq T)) :=
+  match stack with
+  | [::] => [::]
+  | xs :: stack =>
+    (if nilp xs then None else Some (condrev mode xs)) ::
+      astack_of_stack (~~ mode) stack
+  end.
+
+Notation merge := (path.merge leT) (only parsing).
+Notation merge' :=
+  (fun xs ys => rev (path.merge geT (rev ys) (rev xs))) (only parsing).
+Notation flatten_stack :=
+  (foldl (fun xs : seq T => oapp (cat^~ xs) xs)) (only parsing).
+
+Lemma apop_mergeE mode xs stack :
+  Abstract.pop merge merge' mode xs (astack_of_stack mode stack)
+  = pop mode (condrev mode xs) stack.
+Proof.
+have [n] := ubnP (size stack).
+by elim: n mode xs stack => // n IHn [] xs [|[[|[|z zs] stack]|y ys stack]] /=;
+  rewrite ?M.revmergeE ?revK //; try move/(@ltnW _.+2); move=> /IHn ->.
+Qed.
+
+Lemma apush_mergeE xs stack :
+  ~~ nilp xs ->
+  Abstract.push merge merge' xs (astack_of_stack false stack)
+  = astack_of_stack false (push xs stack).
+Proof.
+have [n] := ubnP (size stack).
+by elim: n xs stack => // n IHn xs [|[|y ys] [|[|z zs] stack]] //=;
+  try move=> /(@ltnW _.+2) /IHn ->; try (by case: ifP);
+  rewrite ?M.revmergeE revK /nilp ?(size_rev, size_merge, size_cat).
+Qed.
+
+Lemma asort1_mergeE :
+  Abstract.sort1 leT merge merge' (fun x => [:: x]) [::] =1 sort1.
+Proof.
+rewrite /Abstract.sort1 /sort1 -/(astack_of_stack false [::]) => xs.
+elim: xs (Nil (seq _)) => /= [|x xs IHxs] stack; first exact: apop_mergeE.
+by rewrite -IHxs apush_mergeE.
+Qed.
+
+Lemma asort2_mergeE :
+  Abstract.sort2 leT merge merge' (fun x => [:: x]) [::] =1 sort2.
+Proof.
+move=> xs; have [n] := ubnP (size xs).
+rewrite /Abstract.sort2 /sort2 -/(astack_of_stack false [::]).
+elim: n (Nil (seq _)) xs => // n IHn stack [|x [|x' xs /= /ltnW /IHn <-]] /=;
+  try by rewrite apop_mergeE.
+by rewrite apush_mergeE; last case: ifP.
+Qed.
+
+Lemma asort3_mergeE :
+  Abstract.sort3 leT merge merge' (fun x => [:: x]) [::] =1 sort3.
+Proof.
+move=> xs; have [n] := ubnP (size xs).
+rewrite /Abstract.sort3 /sort3 -/(astack_of_stack false [::]).
+move: n (Nil (seq _)) xs.
+elim=> // n IHn stack [|x [|x' [|x'' xs /= /ltnW /ltnW /IHn <-]]] /=;
+  try by rewrite apop_mergeE.
+rewrite apush_mergeE; last by rewrite /nilp !(size_rev, size_merge).
+by rewrite !(fun_if rev, fun_if (path.merge _ _), fun_if (cons _)).
+Qed.
+
+Lemma asortN_mergeE :
+  Abstract.sortN leT merge merge' (fun x => [:: x]) [::] =1 sortN.
+Proof.
+case=> // x xs; have [n] := ubnP (size xs).
+rewrite /Abstract.sortN /sortN -/(astack_of_stack false [::]).
+elim: n (Nil (seq _)) x xs => // n IHn stack x [|y xs /= /ltnSE Hxs].
+  by rewrite [LHS]apop_mergeE.
+rewrite /Abstract.sortNrec -/(Abstract.incr _ _ _ _) -/(Abstract.decr _ _ _ _).
+pose rs := Nil T; rewrite -{1}[[:: x]]/(rcons (rev rs) x) -/(x :: rs).
+elim: xs Hxs x y rs => [_|z xs IHxs /= /ltnW Hxs] x y rs.
+  rewrite /Abstract.incr /Abstract.decr !apop_mergeE rev_rcons revK /= /geT.
+  by case: leT.
+rewrite /Abstract.incr -/(Abstract.incr _ _ _ _).
+rewrite /Abstract.decr -/(Abstract.decr _ _ _ _) -/(Abstract.sortNrec _ _ _ _).
+move: (IHxs Hxs y z (x :: rs)); rewrite -rev_cons rev_rcons revK /= /geT.
+by do 2 case: leT; rewrite // apush_mergeE ?rev_nilp // IHn.
+Qed.
+
+Lemma apush_catE (xs ys : seq T) stack :
+  flatten_stack ys (Abstract.push cat cat xs stack)
+  = flatten_stack (xs ++ ys) stack.
+Proof.
+have [n] := ubnP (size stack).
+by elim: n xs stack => // n IHn xs [|[zs [|[zs'|] stack]|stack]] //=;
+  try move=> /(@ltnW _.+2) /IHn ->; rewrite !catA.
+Qed.
+
+Lemma apop_catE mode xs stack :
+  Abstract.pop cat cat mode xs stack = flatten_stack xs stack.
+Proof.
+have [n] := ubnP (size stack).
+by elim: n mode xs stack => // n IHn mode xs [|[ys stack|[|[zs|] stack]]] //=;
+  try move/(@ltnW _.+2); move=> /IHn ->; rewrite ?if_same.
+Qed.
+
+Lemma asort1_catE : Abstract.sort1 leT cat cat (fun x => [:: x]) [::] =1 id.
+Proof.
+move=> xs; rewrite /Abstract.sort1 -[RHS]/(flatten_stack xs [::]).
+elim: xs (Nil (option _)) => /= [|x xs IHxs] stack; first exact: apop_catE.
+by rewrite IHxs apush_catE.
+Qed.
+
+Lemma asort2_catE : Abstract.sort2 leT cat cat (fun x => [:: x]) [::] =1 id.
+Proof.
+move=> xs; have [n] := ubnP (size xs).
+rewrite /Abstract.sort2 -[RHS]/(flatten_stack xs [::]).
+move: n (Nil (option _)) xs.
+by elim=> // n IHn stack [|x [|x' xs /= /ltnW /IHn ->]] /=;
+  rewrite (apop_catE, apush_catE).
+Qed.
+
+Lemma asort3_catE : Abstract.sort3 leT cat cat (fun x => [:: x]) [::] =1 id.
+Proof.
+move=> xs; have [n] := ubnP (size xs).
+rewrite /Abstract.sort3 -[RHS]/(flatten_stack xs [::]).
+move: n (Nil (option _)) xs.
+by elim=> // n IHn stack [|x [|x' [|x'' xs /= /ltnW /ltnW /IHn ->]]] /=;
+  rewrite (apop_catE, apush_catE).
+Qed.
+
+Lemma asortN_catE : Abstract.sortN leT cat cat (fun x => [:: x]) [::] =1 id.
+Proof.
+case=> // x xs; have [n] := ubnP (size xs).
+rewrite /Abstract.sortN -[RHS]/(flatten_stack (x :: xs) [::]).
+elim: n x (Nil (option _)) xs => // n IHn x stack [|y xs /= /ltnSE Hxs];
+  first by rewrite [LHS]apop_catE.
+rewrite /Abstract.sortNrec -/(Abstract.incr _ _ _ _) -/(Abstract.decr _ _ _ _).
+pose rs := Nil T; rewrite -[x :: y :: _]/(rs ++ _) -[[:: x]]/(rs ++ _).
+elim: xs Hxs x y rs => [_|z xs IHxs /= /ltnW Hxs] x y rs.
+  by rewrite if_same [LHS]apop_catE -catA.
+rewrite /Abstract.incr -/(Abstract.incr _ _ _ _).
+rewrite /Abstract.decr -/(Abstract.decr _ _ _ _) -/(Abstract.sortNrec _ _ _ _).
+move: (IHxs Hxs y z (rcons rs x)); rewrite IHn // apush_catE -cats1 -!catA /=.
+by case: leT => ->; rewrite if_same.
+Qed.
+
+End CBV.
+
+Definition sort1_stable :=
+  StableSort sort1 Abstract.sort1 Abstract.sort1_R asort1_mergeE asort1_catE.
+Definition sort2_stable :=
+  StableSort sort2 Abstract.sort2 Abstract.sort2_R asort2_mergeE asort2_catE.
+Definition sort3_stable :=
+  StableSort sort3 Abstract.sort3 Abstract.sort3_R asort3_mergeE asort3_catE.
+Definition sortN_stable :=
+  StableSort sortN Abstract.sortN Abstract.sortN_R asortN_mergeE asortN_catE.
 
 End CBV_.
 
@@ -848,7 +981,7 @@ Section StableSortTheory.
 Let lexord (T : Type) (leT leT' : rel T) :=
   [rel x y | leT x y && (leT y x ==> leT' x y)].
 
-Let lexord_total (T : Type) (leT leT' : rel T) :
+Local Lemma lexord_total (T : Type) (leT leT' : rel T) :
   total leT -> total leT' -> total (lexord leT leT').
 Proof.
 move=> leT_total leT'_total x y /=.
@@ -856,7 +989,7 @@ by move: (leT_total x y) (leT'_total x y) => /orP[->|->] /orP[->|->];
   rewrite /= ?implybE ?orbT ?andbT //= (orbAC, orbA) (orNb, orbN).
 Qed.
 
-Let lexord_trans (T : Type) (leT leT' : rel T) :
+Local Lemma lexord_trans (T : Type) (leT leT' : rel T) :
   transitive leT -> transitive leT' -> transitive (lexord leT leT').
 Proof.
 move=> leT_tr leT'_tr y x z /= /andP[lexy leyx] /andP[leyz lezy].
@@ -864,7 +997,7 @@ rewrite (leT_tr _ _ _ lexy leyz); apply/implyP => lezx; move: leyx lezy.
 by rewrite (leT_tr _ _ _ leyz lezx) (leT_tr _ _ _ lezx lexy); exact: leT'_tr.
 Qed.
 
-Let lexordA (T : Type) (leT leT' leT'' : rel T) :
+Local Lemma lexordA (T : Type) (leT leT' leT'' : rel T) :
   lexord leT (lexord leT' leT'') =2 lexord (lexord leT leT') leT''.
 Proof. by move=> x y /=; case: (leT x y) (leT y x) => [] []. Qed.
 
@@ -872,8 +1005,78 @@ Section StableSortTheory_Part1.
 
 Variable (sort : stableSort).
 
+Local Lemma param_asort :
+  StableSort.asort_ty_R (StableSort.asort sort) (StableSort.asort sort).
+Proof. by case: sort. Qed.
+
+Section SortSeq.
+
+Variable (T : Type) (P : {pred T}) (leT : rel T).
+Let geT x y := leT y x.
+
+Local Lemma asort_mergeE :
+  StableSort.asort sort leT (merge leT)
+    (fun xs ys => rev (merge geT (rev ys) (rev xs))) (fun x => [:: x]) [::]
+  =1 sort _ leT.
+Proof. by case: sort. Qed.
+
+Local Lemma asort_catE :
+  StableSort.asort sort leT cat cat (fun x => [:: x]) [::] =1 id.
+Proof. by case: sort. Qed.
+
+Lemma sort_ind (R : seq T -> seq T -> Prop) :
+  (forall xs xs', R xs xs' -> forall ys ys', R ys ys' ->
+     R (cat xs ys) (merge leT xs' ys')) ->
+  (forall xs xs', R xs xs' -> forall ys ys', R ys ys' ->
+     R (cat xs ys) (rev (merge geT (rev ys') (rev xs')))) ->
+  (forall x, R [:: x] [:: x]) -> R [::] [::] ->
+  forall s, R s (sort _ leT s).
+Proof.
+move=> ? ? Hsingleton ? s; rewrite -[s in R s _]asort_catE -asort_mergeE.
+apply: (@param_asort _ _ eq _ _ R) => //.
+- by move=> ? ? -> ? ? ->; apply: bool_R_refl.
+- by move=> ? ? ->; apply: Hsingleton.
+by elim: s; constructor.
+Qed.
+
+Lemma all_sort (s : seq T) : all P (sort _ leT s) = all P s.
+Proof.
+by elim/sort_ind: (sort _ leT s) => // xs xs' IHxs ys ys' IHys;
+  rewrite !(all_rev, all_merge) all_cat IHxs IHys // andbC.
+Qed.
+
+Lemma size_sort (s : seq T) : size (sort _ leT s) = size s.
+Proof.
+by elim/sort_ind: (sort _ leT s) => // xs xs' IHxs ys ys' IHys;
+  rewrite ?size_rev size_merge !size_cat ?size_rev IHxs IHys // addnC.
+Qed.
+
+Lemma sort_nil : sort _ leT [::] = [::].
+Proof. by case: (sort _) (size_sort [::]). Qed.
+
+Lemma pairwise_sort (s : seq T) : pairwise leT s -> sort _ leT s = s.
+Proof.
+elim/sort_ind: (sort _ leT s) => // xs xs' IHxs ys ys' IHys.
+  rewrite pairwise_cat => /and3P[hlr /IHxs -> /IHys ->].
+  by rewrite !allrel_merge.
+rewrite pairwise_cat => /and3P[hlr /IHxs -> /IHys ->].
+by rewrite allrel_merge 1?allrel_rev2 1?allrelC // rev_cat !revK.
+Qed.
+
+Lemma sorted_sort : transitive leT ->
+  forall s : seq T, sorted leT s -> sort _ leT s = s.
+Proof. by move=> leT_tr s; rewrite sorted_pairwise //; apply/pairwise_sort. Qed.
+
+End SortSeq.
+
 Local Lemma param_sort : StableSort.sort_ty_R sort sort.
-Proof. by case: sort => ? param ?; exact: param. Qed.
+Proof.
+move=> T T' T_R leT leT' leT_R xs xs' xs_R; rewrite -!asort_mergeE.
+apply: (@param_asort _ _ T_R _ _ (list_R T_R) _ _ leT_R _ _ (merge_R leT_R));
+  try by do ?constructor.
+move=> ys ys' ys_R zs zs' zs_R; apply/rev_R/merge_R/rev_R/ys_R/rev_R/zs_R.
+by move=> ? ? ? ? ? ?; apply/leT_R.
+Qed.
 
 Lemma map_sort (T T' : Type) (f : T' -> T) (leT' : rel T') (leT : rel T) :
   {mono f : x y / leT' x y >-> leT x y} ->
@@ -886,42 +1089,6 @@ Qed.
 Lemma sort_map (T T' : Type) (f : T' -> T) (leT : rel T) (s : seq T') :
   sort _ leT (map f s) = map f (sort _ (relpre f leT) s).
 Proof. exact/esym/map_sort. Qed.
-
-Section SortSeq.
-
-Variable (T : Type) (P : {pred T}) (leT : rel T).
-
-Variant sort_spec : seq T -> seq T -> Type :=
-  SortSpec (t : StableSort.trace leT) :
-    sort_spec (StableSort.flatten_trace t) (StableSort.sort_trace t).
-
-Local Lemma sortP (s : seq T) : sort_spec s (sort _ leT s).
-Proof.
-by case: sort => ? ? sortP; have [/= t -> ->] := sortP _ leT s; constructor.
-Qed.
-
-Lemma all_sort (s : seq T) : all P (sort _ leT s) = all P s.
-Proof. by case: sortP; exact: StableSort.all_trace. Qed.
-
-Lemma size_sort (s : seq T) : size (sort _ leT s) = size s.
-Proof. case: sortP; exact: StableSort.size_trace. Qed.
-
-Lemma sort_nil : sort _ leT [::] = [::].
-Proof. by case: (sort _) (size_sort [::]). Qed.
-
-Lemma pairwise_sort (s : seq T) : pairwise leT s -> sort _ leT s = s.
-Proof.
-case: {s}sortP; elim=> [b l IHl r IHr|[] [|x [|y s]]] //=; last by case: leT.
-rewrite pairwise_cat => /and3P[hlr /IHl -> /IHr ->].
-rewrite !allrel_merge ?rev_cat ?revK //; first by case: b.
-by rewrite /allrel all_rev [all _ _]allrelC /allrel all_rev.
-Qed.
-
-Lemma sorted_sort : transitive leT ->
-  forall s : seq T, sorted leT s -> sort _ leT s = s.
-Proof. by move=> leT_tr s; rewrite sorted_pairwise //; apply/pairwise_sort. Qed.
-
-End SortSeq.
 
 Lemma sorted_sort_in (T : Type) (P : {pred T}) (leT : rel T) :
   {in P & &, transitive leT} ->
@@ -936,7 +1103,10 @@ Section EqSortSeq.
 Variables (T : eqType) (leT : rel T).
 
 Lemma perm_sort (s : seq T) : perm_eql (sort _ leT s) s.
-Proof. by case: sortP; exact: StableSort.perm_trace. Qed.
+Proof.
+by apply/permPl; elim/sort_ind: (sort _ leT s) => // xs xs' IHxs ys ys' IHys;
+  rewrite 1?perm_rev perm_merge -1?rev_cat 1?perm_rev perm_cat.
+Qed.
 
 Lemma mem_sort (s : seq T) : sort _ leT s =i s.
 Proof. exact/perm_mem/permPl/perm_sort. Qed.
@@ -950,15 +1120,19 @@ Lemma sort_pairwise_stable (T : Type) (leT leT' : rel T) :
   total leT -> forall s : seq T, pairwise leT' s ->
   sorted (lexord leT leT') (sort _ leT s).
 Proof.
-move=> leT_total s; case: {s}sortP; elim=> [b l IHl r IHr|b s] /=.
-  rewrite pairwise_cat => /and3P[hlr /IHl ? /IHr ?].
-  rewrite fun_if ?(rev_sorted, merge_stable_sorted) ?if_same ?allrel_rev2//;
-    do 2 rewrite /allrel ?all_rev StableSort.all_trace [all _ _]allrelC //.
-  by rewrite allrelC.
-move=> sorted_s1 /pairwise_sorted /(conj sorted_s1) /andP.
-case: (b); rewrite -sorted_relI ?rev_sorted;
-  apply: sub_sorted => x y /= /andP[/eqP xy xy']; rewrite ?xy ?xy' ?implybT //.
-by case: (leT _ _) xy (leT_total x y) => //= _ ->.
+move=> leT_total s.
+suff: (forall P, all P s -> all P (sort T leT s)) /\
+        (pairwise leT' s -> sorted (lexord leT leT') (sort T leT s)).
+  by case.
+elim/sort_ind: (sort _ leT s) => // xs xs' [IHxs IHxs'] ys ys' [IHys IHys'];
+  rewrite pairwise_cat; split => [P|/and3P[hlr /IHxs' ? /IHys' ?]].
+- by rewrite all_cat all_merge => /andP[/IHxs -> /IHys ->].
+- apply/merge_stable_sorted => //=.
+  by apply/IHxs; apply/sub_all: hlr => ?; apply/IHys.
+- by rewrite all_cat all_rev all_merge !all_rev => /andP[/IHxs -> /IHys ->].
+- rewrite rev_sorted; apply/merge_stable_sorted; rewrite ?rev_sorted //.
+  rewrite allrel_rev2 allrelC.
+  by apply/IHxs; apply/sub_all: hlr => ?; apply/IHys.
 Qed.
 
 Lemma sort_pairwise_stable_in (T : Type) (P : {pred T}) (leT leT' : rel T) :
@@ -1188,7 +1362,7 @@ by move=> subseq_ts /(sorted_sort sort leT_tr) <-; exact: subseq_sort.
 Qed.
 
 Lemma mem2_sort (s : seq T) (x y : T) :
-    leT x y -> mem2 s x y -> mem2 (sort _ leT s) x y.
+  leT x y -> mem2 s x y -> mem2 (sort _ leT s) x y.
 Proof.
 move=> lexy; rewrite !mem2E => /subseq_sort; rewrite !eq_sort_insert //.
 by case: (_ == _); rewrite //= lexy.
@@ -1232,13 +1406,13 @@ End StableSortTheory_Part2.
 
 End StableSortTheory.
 
-Arguments map_sort                sort {T T' f leT' leT} _ _.
-Arguments sort_map                sort {T T' f leT} s.
 Arguments all_sort                sort {T} P leT s.
 Arguments size_sort               sort {T} leT s.
 Arguments sort_nil                sort {T} leT.
 Arguments pairwise_sort           sort {T leT s} _.
 Arguments sorted_sort             sort {T leT} leT_tr {s} _.
+Arguments map_sort                sort {T T' f leT' leT} _ _.
+Arguments sort_map                sort {T T' f leT} s.
 Arguments sorted_sort_in          sort {T P leT} leT_tr {s} _ _.
 Arguments perm_sort               sort {T} leT s _.
 Arguments mem_sort                sort {T} leT s _.
