theories/param.v
@@ -1,4 +1,4 @@
-From mathcomp Require Import ssreflect ssrfun ssrbool eqtype ssrnat seq.
+From mathcomp Require Import ssreflect ssrfun ssrbool eqtype ssrnat seq path.
 From Param Require Export Param.
 
 Set Implicit Arguments.
@@ -17,6 +17,7 @@ Parametricity eq.
 Parametricity or.
 Parametricity Acc.
 Parametricity bool.
+Parametricity option.
 Parametricity prod.
 Parametricity nat.
 Parametricity list.
@@ -24,6 +25,8 @@ Parametricity pred.
 Parametricity rel.
 Parametricity BinNums.positive.
 Parametricity BinNums.N.
+Parametricity merge.
+Parametricity rev.
 
 Lemma bool_R_refl b1 b2 : b1 = b2 -> bool_R b1 b2.
 Proof. by case: b1 => <-; constructor. Qed.
